compare.v: support for two-way comparisons.

src/compare.v
@@ -1,5 +1,5 @@
 From stdpp Require Import base.
-From marble Require Import tactics wp wp_tactics orders sorting.
+From marble Require Import tactics wp wp_tactics orders sorting bool.
 
 Unset Universe Minimization ToSet.
 Generalizable All Variables.
@@ -7,7 +7,18 @@ Set Universe Polymorphism.
 
 (* -------------------------------------------------------------------------- *)
 
-(* Three-way comparisons. *)
+(* Two-way comparison functions. *)
+
+(* A [leb] function performs a two-way comparison. *)
+
+(* [leb] stands for "Less than or Equal, Boolean". *)
+
+(* [Leb A] means that the type [A] has a [leb] function. *)
+
+Class Leb (A : Type) :=
+  { leb : A → A → bool }.
+
+(* Three-way comparison functions. *)
 
 (* This type exists in the standard library:
 Inductive comparison := Eq | Lt | Gt.
@@ -20,10 +31,11 @@ Inductive comparison := Eq | Lt | Gt.
 Class Compare (A : Type) :=
   { compare : A → A → comparison }.
 
-(* [Comparable A] means that the [compare] function at type [A]
-   is correct with respect to the default preorder on this type. *)
+(* -------------------------------------------------------------------------- *)
 
-Section Comparable.
+(* Specifications for comparison functions. *)
+
+Section Specs.
 
 Open Scope element_scope.
 
@@ -53,12 +65,54 @@ Proof. unfold equivalent. tauto. Qed.
 Lemma gt_ge x y :  x > y → x ≥ y.
 Proof. eauto using lt_le. Qed.
 
+(* [LebSpec A] means that the [leb] function at type [A] is correct
+   with respect to the default preorder on this type. *)
+
+Section LebSpec.
+
+Context `{Leb A}.
+
+Class LebSpec := {
+  leb_spec :
+    ∀ x y : A, isBool (leb x y) (x ≤ y) (x > y)
+}.
+
+(* We make [leb_spec] an instance, so [wp_if] works out of the box. *)
+
+Global Existing Instance leb_spec.
+
+(* This is an example. *)
+
+Local Lemma example `{LebSpec} {B} (x y : A) (e1 e2 : B) (Q : B → Prop) :
+  (x ≤ y → wp e1 Q) →
+  (x > y → wp e2 Q) →
+  wp (if leb x y then e1 else e2) Q.
+Proof.
+  intros. wp_if.
+  + eauto.
+  + eauto.
+Qed.
+
+End LebSpec.
+
+(* [Comparable A] means that the [compare] function at type [A]
+   is correct with respect to the default preorder on this type. *)
+
+(* The assertion [CompareSpec] is defined in the standard library. *)
+
+Section Comparable.
+
 Context `{Compare A}.
 
 Class Comparable := {
   compare_spec :
     ∀ x y : A, CompareSpec (x ≡ y) (x < y) (x > y) (compare x y)
 }.
+
+(* This lemma is useful when a [compare] function is used to perform a
+   two-way comparison. It allows reasoning about each of the two
+   branches just once. However, this programming style is not
+   recommended, as Rocq will silently duplicate one of the branches. *)
 
 Lemma wp_compare_Gt_Le `{Comparable} {B} (x y : A) (e1 e2 : B) (Q : B → Prop) :
   (x > y → wp e1 Q) →
@@ -72,6 +126,8 @@ Proof.
 Qed.
 
 End Comparable.
+
+End Specs.
 
 Global Ltac wp_compare :=
   simple eapply wp_compare_Gt_Le; [ eauto | intro | intro ].
